ArchSemTinyArm/PromisingFirstProof.lean
@@ -6,11 +6,55 @@ open ArchSem.NondeterministicMonad
 open ArchSem.TerminatingModel
 open ArchSemTinyArm.Promising
 
+theorem NEStateM.bind_mono {m₁ m₂ : NEStateM ε σ α} {f₁ f₂ : α → NEStateM ε σ β} {s : σ} {sb : σ × β}
+    : (∀ sa ∈ (m₁ s).oks, sa ∈ (m₂ s).oks)
+    → (∀ sa ∈ (m₁ s).oks, sb ∈ (f₁ sa.snd sa.fst).oks → sb ∈ (f₂ sa.snd sa.fst).oks)
+    → (sb ∈ (Bind.bind m₁ f₁ s).oks → sb ∈ (Bind.bind m₂ f₂ s).oks)
+  := by
+  intro h_m h_f h
+  simp only [Bind.bind] at h ⊢
+  rw [NEStateM.bind_iff'] at h ⊢
+  obtain ⟨sa, h_sa, h⟩ := h
+  refine ⟨sa, h_m sa h_sa, h_f sa h_sa h⟩
+
+theorem NEStateM.bind_mono_right {m : NEStateM ε σ α} {f₁ f₂ : α → NEStateM ε σ β} {s : σ} {sb : σ × β}
+    : (∀ sa ∈ (m s).oks, sb ∈ (f₁ sa.snd sa.fst).oks → sb ∈ (f₂ sa.snd sa.fst).oks)
+    → (sb ∈ (Bind.bind m f₁ s).oks → sb ∈ (Bind.bind m f₂ s).oks)
+  := by
+  intro h_f
+  exact NEStateM.bind_mono (by simp) h_f
+
+theorem NEStateM.bind_mono_left {m₁ m₂ : NEStateM ε σ α} {f : α → NEStateM ε σ β} {s : σ} {sb : σ × β}
+    : (∀ sa ∈ (m₁ s).oks, sa ∈ (m₂ s).oks)
+    → (sb ∈ (Bind.bind m₁ f s).oks → sb ∈ (Bind.bind m₂ f s).oks)
+  := by
+  intro h_m
+  exact NEStateM.bind_mono h_m (by simp)
+
+theorem NEStateM.bind_get_elim {f : σ → NEStateM ε σ β} {s : σ}
+    : Bind.bind get f s = f s s
+  := by
+  simp [
+    bind, get,
+    NEStateM.get, NEStateM.bind,
+    NExcept.pure, NExcept.bind, NExcept.merge
+  ]
+
+theorem NEStateM.bind_modify_elim {f : Unit → NEStateM ε σ β} {h : σ → σ} {s : σ}
+    : Bind.bind (modify h) f s = f () (h s)
+  := by
+  simp [
+    bind, modify, modifyGet,
+    NEStateM.bind, 
+    NExcept.pure, NExcept.bind, NExcept.merge
+  ]
+
 namespace ArchSemTinyArm.Promising
 
 -- Common simplification bundle for NEStateM/NExcept proof scripts.
 open Lean Elab Tactic Lean.Parser.Tactic
 
+/- TODO: remove
 /-
 TODO: This custom tactic is a bit brute force. Lets make it more precise.
 
@@ -25,11 +69,12 @@ elab "simp_nestatem" loc:(location)? : tactic => do
     NEStateM.pure, NEStateM.bind, 
     List.foldr, List.map, List.append_nil
   ] $loc))
+  -/
 
 theorem run_to_termination_monotonic_fuel
-    (tid : Fin nThreads) (initmem : InitialMem) (isem : SailM Unit)
-    (termination : TerminationCondition nThreads)
-    (fuel : Nat) (base : Nat) (promises : List Msg) (pstate : ProjectedModelState)
+    {tid : Fin nThreads} {initmem : InitialMem} {isem : SailM Unit}
+    {termination : TerminationCondition nThreads}
+    {fuel base : Nat} {promises : List Msg} {pstate : ProjectedModelState}
     : ∀ s ∈ (runToTermination tid initmem isem termination fuel base (promises, pstate)).oks,
         s.snd →
         s ∈ (runToTermination tid initmem isem termination (fuel + 1) base (promises, pstate)).oks
@@ -42,27 +87,31 @@ theorem run_to_termination_monotonic_fuel
     contradiction
   | succ f ih =>
     intro s h fuelRemains
-    rw [runToTermination] at h ⊢
-    simp only [Bind.bind] at h ⊢
-    rw [NEStateM.bind_iff] at h ⊢
-    rcases h with ⟨s', a', h_interp, h⟩
-    refine ⟨s', a', h_interp, ?_⟩
-    simp_nestatem at h ⊢
+    revert h
+    rw [runToTermination, runToTermination]
+    apply NEStateM.bind_mono_right
+    intro (s', a') h_interp
+    simp only [NEStateM.bind_get_elim]
+    intro h
     split at h
-    case succ.isFalse h_termination =>
+    case isFalse h_termination =>
       simp only [h_termination, Bool.false_eq_true, ↓reduceIte]
-      simp_nestatem at h ⊢
-      exact ih s'.fst
-        { threadState := s'.snd.threadState, mem := s'.snd.mem, iis := IIS.init }
-        s h fuelRemains
-    case succ.isTrue h_termination =>
+      simp only [NEStateM.bind_modify_elim] at h ⊢
+      exact ih s h fuelRemains
+    case isTrue h_termination =>
       simp only [h_termination, ↓reduceIte]
       assumption
 
+
+/-
+CR clang: This proof is made awkward by the fact that
+runToTermination returns a structre marked with noFuel instead
+of using an except...
+-/
 theorem run_to_termination_stays_terminated
-    (tid : Fin nThreads) (initmem : InitialMem) (isem : SailM Unit)
-    (termination : TerminationCondition nThreads)
-    (fuel : Nat) (base : Nat) (promises₀ : List Msg) (pstate₀ : ProjectedModelState)
+    {tid : Fin nThreads} {initmem : InitialMem} {isem : SailM Unit}
+    {termination : TerminationCondition nThreads}
+    {fuel : Nat} {base : Nat} {promises₀ : List Msg} {pstate₀ : ProjectedModelState}
       : ( ∀ (promises : List Msg) (pstate : ProjectedModelState),
           ((promises, pstate), false)
           ∉ (runToTermination tid initmem isem termination fuel base (promises₀, pstate₀)).oks )
@@ -70,11 +119,21 @@ theorem run_to_termination_stays_terminated
           ((promises, pstate), false)
           ∉ (runToTermination tid initmem isem termination (fuel + 1) base (promises₀, pstate₀)).oks )
   := by
+  -- Apply contrapositive to get in terms of `∃. ∈`
+  intro h
+  simp only [← not_exists] at h ⊢
+  revert h
+  apply mt
+  
   induction fuel generalizing promises₀ pstate₀ with
   | zero =>
     intro h
-    simp [runToTermination, pure, NEStateM.pure, NExcept.pure] at h
+    simp [runToTermination, pure, NEStateM.pure, NExcept.pure]
   | succ f ih =>
+    rw [runToTermination, runToTermination]
+    simp
+    apply NEStateM.bind_mono_right
+    
     intro h promises pstate
     rw [runToTermination] at h ⊢
     simp only [Bind.bind] at h ⊢
@@ -94,13 +153,23 @@ theorem run_to_termination_stays_terminated
     · contradiction
     · assumption
 
-theorem enumerate_result_promises_monotonic_fuel
-    (fuel : Nat) (tid : Fin nThreads) (initmem : InitialMem) (isem : SailM Unit)
-    (termCond : TerminationCondition nThreads) (ts : ThreadState) (mem : PromisingMemory)
-    : ∀ s ∈ (enumerateResults fuel tid initmem isem termCond ts mem).promises,
-        ¬(enumerateResults fuel tid initmem isem termCond ts mem).outOfFuel →
-        s ∈ (enumerateResults (fuel + 1) tid initmem isem termCond ts mem).promises ∧
-        ¬(enumerateResults (fuel + 1) tid initmem isem termCond ts mem).outOfFuel
+theorem enumerate_results_stays_terminated {nThreads : Nat}
+    {fuel : Nat} {tid : Fin nThreads} {initmem : InitialMem} {isem : SailM Unit}
+    {termCond : TerminationCondition nThreads} {ts : ThreadState} {mem : PromisingMemory}
+    : ¬(enumerateResults nThreads fuel tid initmem isem termCond ts mem).outOfFuel →
+      ¬(enumerateResults nThreads (fuel + 1) tid initmem isem termCond ts mem).outOfFuel
+  := by
+  simp only [enumerateResults, List.any_eq_true, Bool.not_eq_eq_eq_not, Bool.not_true, Prod.exists,
+    exists_eq_right, not_exists]
+  apply run_to_termination_stays_terminated
+
+theorem enumerate_result_promises_monotonic_fuel {nThreads : Nat}
+    {fuel : Nat} {tid : Fin nThreads} {initmem : InitialMem} {isem : SailM Unit}
+    {termCond : TerminationCondition nThreads} {ts : ThreadState} {mem : PromisingMemory}
+    : ∀ s ∈ (enumerateResults nThreads fuel tid initmem isem termCond ts mem).promises,
+        ((enumerateResults nThreads fuel tid initmem isem termCond ts mem).outOfFuel = false) →
+        s ∈ (enumerateResults nThreads (fuel + 1) tid initmem isem termCond ts mem).promises ∧
+        ((enumerateResults nThreads (fuel + 1) tid initmem isem termCond ts mem).outOfFuel = false)
   := by
   intro s
   simp only [enumerateResults]
@@ -116,17 +185,24 @@ theorem enumerate_result_promises_monotonic_fuel
       exists promises
       refine ⟨?_, h_s_in_promises⟩
       exists pmstate
-      have := run_to_termination_monotonic_fuel tid initmem isem termCond fuel
-        (List.length mem) [] { threadState := ts, mem := mem, iis := IIS.init }
-        ((promises, pmstate), true) h
-      simp [this]
+      exact Or.inr (run_to_termination_monotonic_fuel _ h (by simp))
     case right =>
-      exact run_to_termination_stays_terminated tid initmem isem termCond fuel (List.length mem)
-        [] { threadState := ts, mem := mem, iis := IIS.init } h_fuel_remains
+      exact run_to_termination_stays_terminated h_fuel_remains
+
+theorem enumerate_results_eual {nThreads : Nat}
+    {fuel : Nat} {tid : Fin nThreads} {initmem : InitialMem} {isem : SailM Unit}
+    {termCond : TerminationCondition nThreads} {ts : ThreadState} {mem : PromisingMemory}
+    : ((enumerateResults nThreads fuel tid initmem isem termCond ts mem).outOfFuel = false) →
+      (enumerateResults nThreads fuel tid initmem isem termCond ts mem)
+      = (enumerateResults nThreads (fuel + 1) tid initmem isem termCond ts mem)
+  := by
+  intro h_fuel
+  simp only [enumerateResults]
+  sorry
 
 theorem promise_select_tid_monotonic_fuel
-    (fuel : Nat) (mstate : ModelState nThreads) (tid : Fin nThreads) (isem : SailM Unit)
-    (termCond : TerminationCondition nThreads)
+    {fuel : Nat} {mstate : ModelState nThreads} {tid : Fin nThreads} {isem : SailM Unit}
+    {termCond : TerminationCondition nThreads}
     : ∀ s ∈ (promiseSelectTid fuel mstate tid isem termCond).oks,
         s ∈ (promiseSelectTid (fuel + 1) mstate tid isem termCond).oks
   := by
@@ -134,54 +210,123 @@ theorem promise_select_tid_monotonic_fuel
   intro msg h
   split at h <;> try contradiction
   rename_i h_is_false
-  obtain ⟨h_l, h_r⟩ := enumerate_result_promises_monotonic_fuel fuel tid mstate.initmem
-    isem termCond mstate.threadStates[tid] mstate.mem msg h h_is_false
+  simp only [Bool.not_eq_true] at h_is_false
+  obtain ⟨h_l, h_r⟩ := enumerate_result_promises_monotonic_fuel msg h h_is_false
   simp only [h_r, Bool.false_eq_true, ↓reduceIte, NExcept.choose, h_l]
 
 theorem run_step_monotonic_fuel
-   (fuel : Nat) (isem : SailM Unit) (termCond : TerminationCondition nThreads)
-   (pState : ModelState nThreads)
-   : ∀ s ∈ (runStep fuel isem termCond pState).oks,
-       s ∈ (runStep (fuel + 1) isem termCond pState).oks
- := by
- simp only [runStep, promiseTid]
- intro (mstate, ()) h
- simp only [Bind.bind, NEStateM.bind_iff] at h ⊢
- rcases h with ⟨s₁, s₂, h_get, s₃, tid, h_choose, h⟩
- exists s₁, s₂, h_get, s₃, tid, h_choose
- split at h <;> try contradiction
- rename_i h_terminated
- simp only [h_terminated, Bool.false_eq_true, ↓reduceIte]
- simp only [NEStateM.bind_iff, Fin.exists_fin_two, Fin.isValue] at h ⊢
- rcases h with ⟨s₁, h⟩
- exists s₁
- rcases h with ⟨h_get₁, s₂, s₃, h_get₂, s₄, msg, h_prom, h_mod⟩ | ⟨h⟩
- case inl =>
-   apply Or.inl
-   refine ⟨h_get₁, s₂, s₃, h_get₂, s₄, msg, ?_⟩
-   simp only [liftM, monadLift, MonadLift.monadLift, List.mem_map,
-     Prod.mk.injEq, exists_eq_right_right] at h_prom ⊢
-   have := promise_select_tid_monotonic_fuel fuel s₃ tid isem termCond msg h_prom.1
-   simp [this, h_prom.2, h_mod]
- case inr =>
-   exact Or.inr h
+    {fuel : Nat} {isem : SailM Unit} {termCond : TerminationCondition nThreads}
+    {pState : ModelState nThreads}
+    : ∀ s ∈ (runStep fuel isem termCond pState).oks,
+        s ∈ (runStep (fuel + 1) isem termCond pState).oks
+  := by
+  simp only [runStep, promiseTid]
+  intro (mstate, ())
+
+  apply NEStateM.bind_mono_right
+  intro (s₁, s₂) h_get
+  apply NEStateM.bind_mono_right
+  intro (s₃, tid) h_choose
+
+  intro h
+  split at h <;> try contradiction
+  rename_i h_terminated
+
+  revert h
+  simp only [h_terminated, Bool.false_eq_true, ↓reduceIte]
+  apply NEStateM.bind_mono_right
+  intro (s₁, choice) h_choice
+
+  match choice with
+  | 0 =>
+    simp only [NEStateM.bind_get_elim]
+    apply NEStateM.bind_mono_left
+    simp only [liftM, monadLift, MonadLift.monadLift]
+    simp only [List.mem_map, forall_exists_index, and_imp, forall_apply_eq_imp_iff₂, Prod.mk.injEq,
+      true_and, exists_eq_right]
+    apply promise_select_tid_monotonic_fuel
+  | 1 =>
+    simp []
 
 -- TODO: be consistent with pstate/pState naming.
 
-theorem naive_runtime_monotonic_fuel
-    : ∀ (pState : ModelState nThreads) (fuel : Nat),
-      ∀ r ∈ (runNaive fuel isem nThreads termCond pState).oks,
+theorem naive_runtime_monotonic_fuel {fuel : Nat} {isem : SailM Unit} {nThreads : Nat}
+    {termCond : TerminationCondition nThreads} {pState : ModelState nThreads} 
+    : ∀ r ∈ (runNaive fuel isem nThreads termCond pState).oks,
         r ∈ (runNaive (fuel + 1) isem nThreads termCond pState).oks
   := by
-  intro pState fuel (promises, mstate) h
+  intro (promises, mstate)
   induction fuel generalizing pState with
-  | zero => contradiction
+  | zero =>
+    rw [runNaive]
+    intros
+    contradiction
   | succ f ih =>
-    rw [runNaive] at h ⊢
+    rw [runNaive, runNaive]
+
+    apply NEStateM.bind_mono_right
+    intro (s₁, s₂) h_get
+    
+    split
+    case isFalse h_term =>
+      apply NEStateM.bind_mono
+      · apply run_step_monotonic_fuel
+      · intro pState _ ; apply ih
+    case isTrue h_term =>
+      simp
+
+theorem promise_first_runtime_monotonic_fuel {fuel : Nat} {isem : SailM Unit} {nThreads : Nat}
+    {termCond : TerminationCondition nThreads} {pState : ModelState nThreads} 
+    : ∀ r ∈ (runPromiseFirst fuel isem nThreads termCond pState).oks,
+        r ∈ (runPromiseFirst (fuel + 1) isem nThreads termCond pState).oks
+  := by
+  intro (promises, mstate) h
+  induction fuel generalizing pState with
+  | zero =>
+    rw [runPromiseFirst] at h
+    contradiction
+  | succ f ih =>
+    rw [runPromiseFirst] at h ⊢
+    simp only [Nat.reduceBeqDiff, Bool.false_eq_true, ↓reduceIte] at h ⊢
     simp only [Bind.bind, NEStateM.bind_iff] at h ⊢
-    rcases h with ⟨s₁, s₂, h_get, h⟩
-    refine ⟨s₁, s₂, h_get, ?_⟩
-    split at h
+    rcases h with ⟨s₁, s_enum, h_get, h⟩
+    refine ⟨s₁, s_enum, h_get, ?_⟩
+    split at h <;> try contradiction
+    split <;> rename_i h_fuel h_fuel'
+    <;> simp only [Nat.add_one_sub_one, Fin.getElem_fin, Vector.any_toList, Vector.any_eq_true,
+          Vector.getElem_ofFn, not_exists, Bool.not_eq_true, Vector.any_eq_true] at h_fuel h_fuel'
+    case isTrue =>
+      rcases h_fuel' with ⟨tid, h_tid, h_fuel'⟩
+      specialize h_fuel tid h_tid
+      apply absurd h_fuel'
+      apply enumerate_results_stays_terminated
+      simp [h_fuel]
+    case isFalse =>
+      simp only [NEStateM.bind_iff] at h ⊢
+      rcases h with ⟨s₁, u, h_u, s_match, c, h_c, h⟩
+      refine ⟨s₁, u, h_u, s_match, c, h_c, ?_⟩
+      split at h
+      case h_1 => -- make promise
+        simp only [NEStateM.bind_iff] at h ⊢
+        rcases h with ⟨s₁, tid, h_choose_tid, s₂, msg, h_choose_ev, s₃, u, h_mod, h⟩
+        refine ⟨s₁, tid, h_choose_tid, s₂, msg, ?_⟩
+        simp only [NEStateM.choose, NExcept.choose] at h_choose_ev ⊢
+        simp only [Nat.add_one_sub_one, List.mem_map, Prod.mk.injEq, exists_eq_right_right] at h_choose_ev ⊢
+        simp only [Fin.getElem_fin, Vector.getElem_ofFn, Fin.eta] at h_choose_ev ⊢
+        specialize h_fuel tid.val tid.isLt
+        -- TODO: maybe I should make theorem arguments implicit
+        have := enumerate_result_promises_monotonic_fuel _ h_choose_ev.left h_fuel
+        exact ⟨⟨this.left, h_choose_ev.right⟩, s₃, u, h_mod, ih h⟩
+      case h_2 => -- terminate
+        simp only [NEStateM.bind_iff] at h ⊢
+        rcases h with ⟨s₁, threads, h_enumerate, h⟩
+        -- TODO: Here I need to use enumerate_result_final_states_equal
+        -- the order matters because we use mapM
+        -- Or maybe just write theorem for enumerate_results_equal
+        have := enumerate_result_promises_monotonic_fuel
+        refine ⟨s₁, threads, h_enumerate, ?_⟩
+      case h_3 => -- 
+      
     case isFalse h_term =>
       simp only [h_term, ↓reduceDIte]
       rw [NEStateM.bind_iff] at h ⊢
@@ -191,5 +336,32 @@ theorem naive_runtime_monotonic_fuel
       exact ⟨s₃, u, h_l, h_r⟩
     case isTrue h_term =>
       simp [h_term, h]
+
+theorem naive_model_monotonic_fuel {isem : SailM Unit} {fuel : Nat}
+    : (createNaiveModel isem fuel).weaker (createNaiveModel isem (fuel + 1))
+  := by
+  rw [ComputationalTerminatingModel.weaker]
+  intro nThreads termCond init final t r h r_eq
+  rw [createNaiveModel, promisingRuntimeToModel, r_eq] at h ⊢
+  simp only [List.mem_append, List.mem_map, reduceCtorEq, and_false, exists_false, false_or] at h ⊢
+  simp only [List.mem_eraseDups, List.mem_map] at h ⊢
+  rcases h with ⟨r, h, h_eq⟩
+  refine ⟨r, ?_, h_eq⟩
+  apply naive_runtime_monotonic_fuel
+  exact h
+
+theorem naive_monotonic_fuel_full {isem : SailM Unit} {fuel : Nat}
+    : ∀ fuel' ≥ fuel,
+    (createNaiveModel isem fuel).weaker (createNaiveModel isem (fuel' + 1))
+  := by
+  intro fuel' h
+  let d := fuel' - fuel
+  have h_fuel'_eq : fuel' = fuel + d := by omega
+  rw [h_fuel'_eq]
+  induction d with
+  | zero =>
+    exact naive_model_monotonic_fuel
+  | succ k ih =>
+    exact ComputationalTerminatingModel.weaker_transitive ih naive_model_monotonic_fuel
 
 end ArchSemTinyArm.Promising
